Fix Hoare/ModSem to compile

lib/Any.v
@@ -7,12 +7,18 @@ Module Type AnyType.
 
   Parameter t: Type.
   Parameter upcast: forall {T: Type}, T -> t.
-  (* Parameter downcast: forall {T: Type}, t -> option T. *)
+  Parameter downcast: forall {T: Type}, t -> option T.
 
   Parameter upcast_inj: forall A B (a: A) (b: B) (EQ: upcast a = upcast b),
       <<EQ: A = B>> /\ <<EQ: a ~= b>>.
   Parameter upcast_surj: forall A B a b (EQ: A = B) (EQ: a ~= b),
       <<EQ: @upcast A a = @upcast B b>>.
+
+  Parameter upcast_downcast: forall T (a: T), downcast (upcast a) = Some a.
+
+  (* Parameter patmat: forall R (body: forall (T: Type), T -> R), t -> R. *)
+  (* Parameter patmat_spec: forall R (body: forall (T: Type), T -> R) *)
+  (*                               T (t: T), (patmat body (upcast t): R) = body _ t. *)
 
 End AnyType.
 
@@ -26,12 +32,12 @@ Module Any: AnyType.
   Arguments _upcast {ty}.
   Arguments upcast {ty}.
 
-  (* Definition downcast {T: Type} (a: t): option T. *)
-  (*   destruct a. *)
-  (*   destruct (excluded_middle_informative (ty0 = T)). *)
-  (*   - subst. apply Some. assumption. *)
-  (*   - apply None. *)
-  (* Defined. *)
+  Definition downcast {T: Type} (a: t): option T.
+    destruct a.
+    destruct (excluded_middle_informative (ty0 = T)).
+    - subst. apply Some. assumption.
+    - apply None.
+  Defined.
 
   (* Lemma downcast_elim *)
   (*       a T (v: T) *)
@@ -44,26 +50,26 @@ Module Any: AnyType.
   (*   simpl_depind. eauto. *)
   (* Qed. *)
 
-  (* Lemma downcast_intro *)
-  (*       a T (v: T) *)
-  (*       (TY: a.(ty) = T) *)
-  (*       (VAL: a.(val) ~= v) *)
-  (*   : *)
-  (*     <<CAST: downcast a = Some v>> *)
-  (* . *)
-  (* Proof. *)
-  (*   unfold downcast in *. des_ifs. ss. *)
-  (*   dependent destruction e. ss. *)
-  (* Qed. *)
+  Lemma downcast_intro
+        a T (v: T)
+        (TY: a.(ty) = T)
+        (VAL: a.(val) ~= v)
+    :
+      <<CAST: downcast a = Some v>>
+  .
+  Proof.
+    unfold downcast in *. des_ifs. ss.
+    dependent destruction e. ss.
+  Qed.
 
-  (* Lemma upcast_downcast *)
-  (*       T (a: T) *)
-  (*   : *)
-  (*     downcast (upcast a) = Some a *)
-  (* . *)
-  (* Proof. *)
-  (*   eapply downcast_intro; ss. *)
-  (* Qed. *)
+  Lemma upcast_downcast
+        T (a: T)
+    :
+      downcast (upcast a) = Some a
+  .
+  Proof.
+    eapply downcast_intro; ss.
+  Qed.
 
   (* Lemma upcast_downcast_adjoint *)
   (*       (a: t) T (t: T) *)
@@ -138,6 +144,12 @@ Module Any: AnyType.
       <<EQ: @upcast A a = @upcast B b>>
   .
   Proof. clarify. Qed.
+
+  (* Definition patmat: forall R (body: forall (T: Type), T -> R), t -> R. *)
+  (*   i. destruct X. apply (body ty0 val0). Defined. *)
+  (* Lemma patmat_spec: forall R (body: forall (T: Type), T -> R) *)
+  (*                           T (t: T), (patmat body (upcast t): R) = body _ t. *)
+  (* Proof. ss. Qed. *)
 
 End Any.
 
